verify (and fix) the bytecode implementing fromList
adds an assumption to the prim1_to_bc_thm saying that the code must
contain the primitives (in this case only one primitive, for fromList)
at the expected labels. this assumption will probably carry throughout
this file and need to be satisfied higher up when the initial bytecode
state is created.

compiler/proofs/bytecodeProofScript.sml
@@ -1220,6 +1220,9 @@ val do_Ceq_to_bc_equal = Q.prove (
   (helper_tac >> fs[EVERY2_EVERY] >> metis_tac []) >-
   (helper_tac >> fs[EVERY2_EVERY] >> metis_tac []) >-
   (helper_tac >> fs[EVERY2_EVERY]) >-
+  (helper_tac >> fs[EVERY2_EVERY]) >-
+  (helper_tac >> fs[EVERY2_EVERY]) >-
+  (helper_tac >> fs[EVERY2_EVERY]) >-
   helper_tac >-
   helper_tac >-
   helper_tac >-
@@ -1410,9 +1413,286 @@ val is_Label_prim1_to_bc = store_thm("is_Label_prim1_to_bc",
   Cases >> rw[])
 val _ = export_rewrites["is_Label_prim1_to_bc"]
 
+val contains_primitives_def = Define`
+  contains_primitives code ⇔
+  ∃bc0 bc1.
+    code = bc0 ++ VfromListCode ++ bc1 ∧
+    ALL_DISTINCT (FILTER is_Label code)`
+
+fun next_addr_tac n =
+    match_mp_tac bc_fetch_next_addr >> simp[Abbr`bs1`] >>
+    qexists_tac`bc0 ++ (DROP 2 (TAKE ^(Term n) VfromListCode))` >>
+    simp[VfromListCode_def] >>
+    REWRITE_TAC[SUM_APPEND,FILTER_APPEND,MAP_APPEND] >>
+    EVAL_TAC >> simp[]
+
+val VfromListCode_aux_correct = prove(
+  ``∀vl ls bs bc0 bc1 bvl st cnt pp loopcode.
+      loopcode = DROP 2 (TAKE 20 VfromListCode) ∧
+      bs.code = bc0 ++ loopcode ++ bc1 ∧
+      ALL_DISTINCT (FILTER is_Label bs.code) ∧
+      bs.stack = Number cnt::bvl::st ∧
+      bs.pc = next_addr bs.inst_length bc0 ∧
+      Cv_bv pp vl bvl ∧
+      CvFromList vl = SOME ls
+      ⇒
+      ∃bls.
+      let bs' = bs with <| pc := next_addr bs.inst_length (bc0++loopcode);
+                           stack := Number (cnt + &LENGTH ls)::(REVERSE bls)++st |> in
+      bc_next^* bs bs' ∧
+      LIST_REL (Cv_bv pp) ls bls``,
+  ho_match_mp_tac CvFromList_ind >>
+  simp[CvFromList_def] >>
+  conj_tac >- (
+    rw[Cv_bv_cases_conv] >>
+    srw_tac[DNF_ss][Once RTC_CASES1] >> disj2_tac >>
+    `bc_fetch bs = SOME (Stack (Load 1))` by (
+      match_mp_tac bc_fetch_next_addr >>
+      qexists_tac`bc0++[Label(VfromListLab+1)]` >> simp[] >>
+      simp[FILTER_APPEND,SUM_APPEND] >>
+      simp[VfromListCode_def] ) >>
+    simp[bc_eval1_thm,bc_eval1_def,bump_pc_def,bc_eval_stack_def] >>
+    qho_match_abbrev_tac`bc_next^* bs1 bs2` >>
+    srw_tac[DNF_ss][Once RTC_CASES1] >> disj2_tac >>
+    `bc_fetch bs1 = SOME (Stack (TagEq (block_tag+nil_tag)))` by (
+      match_mp_tac bc_fetch_next_addr >> simp[Abbr`bs1`] >>
+      qexists_tac`bc0 ++ (DROP 2 (TAKE 4 VfromListCode))` >>
+      simp[VfromListCode_def] >>
+      simp[SUM_APPEND,FILTER_APPEND] ) >>
+    simp[bc_eval1_thm,bc_eval1_def,bump_pc_def,bc_eval_stack_def,Abbr`bs1`] >>
+    qho_match_abbrev_tac`bc_next^* bs1 bs2` >>
+    `bc_fetch bs1 = SOME (JumpIf (Lab (VfromListLab+2)))` by (
+      match_mp_tac bc_fetch_next_addr >> simp[Abbr`bs1`] >>
+      qexists_tac`bc0 ++ (DROP 2 (TAKE 5 VfromListCode))` >>
+      simp[VfromListCode_def] >>
+      simp[SUM_APPEND,FILTER_APPEND] ) >>
+    srw_tac[DNF_ss][Once RTC_CASES1] >> disj2_tac >>
+    simp[bc_eval1_thm,bc_eval1_def,Abbr`bs1`,PULL_EXISTS] >>
+    qexists_tac`next_addr bs.inst_length (bc0 ++ DROP 2 (TAKE 19 VfromListCode))` >>
+    conj_tac >- (
+      simp[bc_find_loc_def] >>
+      match_mp_tac bc_find_loc_aux_ALL_DISTINCT >>
+      qexists_tac`LENGTH bc0 + 16` >>
+      rfs[] >>
+      simp[VfromListCode_def,EL_APPEND1,EL_APPEND2] >>
+      simp[TAKE_APPEND1,TAKE_APPEND2] >>
+      REWRITE_TAC[FILTER_APPEND] >>
+      EVAL_TAC ) >>
+    match_mp_tac RTC_SUBSET >>
+    qho_match_abbrev_tac`bc_next bs1 bs2` >>
+    `bc_fetch bs1 = SOME (Stack (Pops 1))` by (
+      match_mp_tac bc_fetch_next_addr >>
+      simp[Abbr`bs1`] >>
+      CONV_TAC SWAP_EXISTS_CONV >>
+      qexists_tac`bc1` >>
+      simp[VfromListCode_def] ) >>
+    simp[bc_eval1_thm,bc_eval1_def,Abbr`bs1`,bc_eval_stack_def,bump_pc_def] >>
+    simp[Abbr`bs2`,bc_state_component_equality] >>
+    simp[VfromListCode_def] >>
+    REWRITE_TAC[SUM_APPEND,FILTER_APPEND,MAP_APPEND] >>
+    EVAL_TAC >> simp[]) >>
+  rw[] >>
+  Cases_on`CvFromList vl`>>fs[]>>rw[]>>
+  simp[PULL_EXISTS] >>
+  srw_tac[DNF_ss][Once RTC_CASES1] >> disj2_tac >>
+  `bc_fetch bs = SOME (Stack (Load 1))` by (
+    match_mp_tac bc_fetch_next_addr >>
+    qexists_tac`bc0++[Label(VfromListLab+1)]` >> simp[] >>
+    simp[FILTER_APPEND,SUM_APPEND] >>
+    simp[VfromListCode_def] ) >>
+  simp[bc_eval1_thm,bc_eval1_def,bump_pc_def,bc_eval_stack_def] >>
+  qho_match_abbrev_tac`∃v vs. bc_next^* bs1 (bs2 v vs) ∧ P v vs` >>
+  srw_tac[DNF_ss][Once RTC_CASES1] >> disj2_tac >>
+  `bc_fetch bs1 = SOME (Stack (TagEq (block_tag+nil_tag)))` by (next_addr_tac`4`) >>
+  fs[Cv_bv_cases_conv] >> rw[] >>
+  simp[bc_eval1_thm,bc_eval1_def,bump_pc_def,bc_eval_stack_def,Abbr`bs1`] >>
+  `cons_tag ≠ nil_tag` by EVAL_TAC >> simp[] >> pop_assum kall_tac >>
+  qho_match_abbrev_tac`∃v vs. bc_next^* bs1 (bs2 v vs) ∧ P v vs` >>
+  `bc_fetch bs1 = SOME (JumpIf (Lab (VfromListLab+2)))` by (next_addr_tac`5`) >>
+  srw_tac[DNF_ss][Once RTC_CASES1] >> disj2_tac >>
+  simp[bc_eval1_thm,bc_eval1_def,Abbr`bs1`,PULL_EXISTS] >>
+  CONV_TAC(RESORT_EXISTS_CONV(sort_vars["n"])) >>
+  qexists_tac`next_addr bs.inst_length (bc0 ++ DROP 2 (TAKE 19 VfromListCode))` >>
+  simp[RIGHT_EXISTS_AND_THM] >>
+  conj_tac >- (
+    simp[bc_find_loc_def] >>
+    match_mp_tac bc_find_loc_aux_ALL_DISTINCT >>
+    qexists_tac`LENGTH bc0 + 16` >>
+    rfs[] >>
+    simp[VfromListCode_def,EL_APPEND1,EL_APPEND2] >>
+    simp[TAKE_APPEND1,TAKE_APPEND2] >>
+    REWRITE_TAC[FILTER_APPEND] >>
+    EVAL_TAC ) >>
+  simp[bump_pc_with_stack] >>
+  fs[bump_pc_def,bc_fetch_with_stack] >>
+  qho_match_abbrev_tac`∃v vs. bc_next^* bs1 (bs2 v vs) ∧ P v vs` >>
+  `bc_fetch bs1 = SOME (Stack (PushInt 1))` by (next_addr_tac`6`) >>
+  srw_tac[DNF_ss][Once RTC_CASES1] >> disj2_tac >>
+  simp[bc_eval1_thm,bc_eval1_def,Abbr`bs1`,bc_eval_stack_def,bump_pc_def] >>
+  ntac 3 (pop_assum kall_tac) >>
+  qho_match_abbrev_tac`∃v vs. bc_next^* bs1 (bs2 v vs) ∧ P v vs` >>
+  `bc_fetch bs1 = SOME (Stack Add)` by (next_addr_tac`7`) >>
+  srw_tac[DNF_ss][Once RTC_CASES1] >> disj2_tac >>
+  simp[bc_eval1_thm,bc_eval1_def,Abbr`bs1`,bc_eval_stack_def,bump_pc_def] >>
+  pop_assum kall_tac >>
+  qho_match_abbrev_tac`∃v vs. bc_next^* bs1 (bs2 v vs) ∧ P v vs` >>
+  `bc_fetch bs1 = SOME (Stack (Load 1))` by (next_addr_tac`8`) >>
+  srw_tac[DNF_ss][Once RTC_CASES1] >> disj2_tac >>
+  simp[bc_eval1_thm,bc_eval1_def,Abbr`bs1`,bc_eval_stack_def,bump_pc_def] >>
+  pop_assum kall_tac >>
+  qho_match_abbrev_tac`∃v vs. bc_next^* bs1 (bs2 v vs) ∧ P v vs` >>
+  `bc_fetch bs1 = SOME (Stack (El 1))` by (next_addr_tac`9`) >>
+  srw_tac[DNF_ss][Once RTC_CASES1] >> disj2_tac >>
+  simp[bc_eval1_thm,bc_eval1_def,Abbr`bs1`,bc_eval_stack_def,bump_pc_def] >>
+  pop_assum kall_tac >>
+  qho_match_abbrev_tac`∃v vs. bc_next^* bs1 (bs2 v vs) ∧ P v vs` >>
+  `bc_fetch bs1 = SOME (Stack (Load 2))` by (next_addr_tac`10`) >>
+  srw_tac[DNF_ss][Once RTC_CASES1] >> disj2_tac >>
+  simp[bc_eval1_thm,bc_eval1_def,Abbr`bs1`,bc_eval_stack_def,bump_pc_def] >>
+  pop_assum kall_tac >>
+  qho_match_abbrev_tac`∃v vs. bc_next^* bs1 (bs2 v vs) ∧ P v vs` >>
+  `bc_fetch bs1 = SOME (Stack (El 0))` by (next_addr_tac`11`) >>
+  srw_tac[DNF_ss][Once RTC_CASES1] >> disj2_tac >>
+  simp[bc_eval1_thm,bc_eval1_def,Abbr`bs1`,bc_eval_stack_def,bump_pc_def] >>
+  pop_assum kall_tac >>
+  qho_match_abbrev_tac`∃v vs. bc_next^* bs1 (bs2 v vs) ∧ P v vs` >>
+  `bc_fetch bs1 = SOME (Stack (Store 2))` by (next_addr_tac`12`) >>
+  srw_tac[DNF_ss][Once RTC_CASES1] >> disj2_tac >>
+  simp[bc_eval1_thm,bc_eval1_def,Abbr`bs1`,bc_eval_stack_def,bump_pc_def] >>
+  pop_assum kall_tac >>
+  qho_match_abbrev_tac`∃v vs. bc_next^* bs1 (bs2 v vs) ∧ P v vs` >>
+  `bc_fetch bs1 = SOME (Stack (Load 0))` by (next_addr_tac`13`) >>
+  srw_tac[DNF_ss][Once RTC_CASES1] >> disj2_tac >>
+  simp[bc_eval1_thm,bc_eval1_def,Abbr`bs1`,bc_eval_stack_def,bump_pc_def] >>
+  pop_assum kall_tac >>
+  qho_match_abbrev_tac`∃v vs. bc_next^* bs1 (bs2 v vs) ∧ P v vs` >>
+  `bc_fetch bs1 = SOME (Stack (Load 2))` by (next_addr_tac`14`) >>
+  srw_tac[DNF_ss][Once RTC_CASES1] >> disj2_tac >>
+  simp[bc_eval1_thm,bc_eval1_def,Abbr`bs1`,bc_eval_stack_def,bump_pc_def] >>
+  pop_assum kall_tac >>
+  qho_match_abbrev_tac`∃v vs. bc_next^* bs1 (bs2 v vs) ∧ P v vs` >>
+  `bc_fetch bs1 = SOME (Stack (Store 1))` by (next_addr_tac`15`) >>
+  srw_tac[DNF_ss][Once RTC_CASES1] >> disj2_tac >>
+  simp[bc_eval1_thm,bc_eval1_def,Abbr`bs1`,bc_eval_stack_def,bump_pc_def] >>
+  pop_assum kall_tac >>
+  qho_match_abbrev_tac`∃v vs. bc_next^* bs1 (bs2 v vs) ∧ P v vs` >>
+  `bc_fetch bs1 = SOME (Stack (Store 1))` by (next_addr_tac`16`) >>
+  srw_tac[DNF_ss][Once RTC_CASES1] >> disj2_tac >>
+  simp[bc_eval1_thm,bc_eval1_def,Abbr`bs1`,bc_eval_stack_def,bump_pc_def] >>
+  pop_assum kall_tac >>
+  qho_match_abbrev_tac`∃v vs. bc_next^* bs1 (bs2 v vs) ∧ P v vs` >>
+  `bc_fetch bs1 = SOME (Jump (Lab (VfromListLab + 1)))` by (next_addr_tac`17`) >>
+  srw_tac[DNF_ss][Once RTC_CASES1] >> disj2_tac >>
+  simp[bc_eval1_thm,bc_eval1_def,Abbr`bs1`,PULL_EXISTS] >>
+  pop_assum kall_tac >>
+  CONV_TAC(RESORT_EXISTS_CONV(sort_vars["n"])) >>
+  qexists_tac`next_addr bs.inst_length bc0` >>
+  simp[RIGHT_EXISTS_AND_THM] >>
+  conj_tac >- (
+    simp[bc_find_loc_def] >>
+    match_mp_tac bc_find_loc_aux_ALL_DISTINCT >>
+    qexists_tac`LENGTH bc0` >>
+    rfs[] >>
+    simp[VfromListCode_def,EL_APPEND1,EL_APPEND2] >>
+    simp[TAKE_APPEND1,TAKE_APPEND2]) >>
+  qho_match_abbrev_tac`∃v vs. bc_next^* bs1 (bs2 v vs) ∧ P v vs` >>
+  first_x_assum(qspecl_then[`bs1`,`bc0`]mp_tac) >>
+  rfs[] >> simp[Abbr`bs1`] >>
+  disch_then(qspec_then`pp`mp_tac) >> simp[] >>
+  strip_tac >>
+  srw_tac[DNF_ss][Once RTC_CASES_RTC_TWICE] >>
+  first_assum(match_exists_tac o concl) >> simp[] >>
+  srw_tac[DNF_ss][Once RTC_CASES1] >> disj1_tac >>
+  simp[bc_state_component_equality,Abbr`bs2`,arithmeticTheory.ADD1] >>
+  conj_tac >- intLib.COOPER_TAC >>
+  simp[Abbr`P`])
+
+val VfromListCode_correct = prove(
+  ``∀bs. contains_primitives bs.code ⇒
+      ∀vl st bvl ls pp.
+      bc_fetch bs = SOME (Call (Lab VfromListLab)) ∧
+      bs.stack = bvl::st ∧
+      Cv_bv pp vl bvl ∧
+      CvFromList vl = SOME ls
+      ⇒
+      ∃bls.
+      let bs' = bump_pc bs with stack := Block vector_tag bls :: st in
+      bc_next^* bs bs' ∧
+      LIST_REL (Cv_bv pp) ls bls``,
+  simp[] >> rw[] >>
+  srw_tac[DNF_ss][Once RTC_CASES1] >> disj2_tac >>
+  simp[bc_eval1_thm,bc_eval1_def] >>
+  fs[contains_primitives_def,bc_find_loc_def] >>
+  simp[PULL_EXISTS] >> CONV_TAC SWAP_EXISTS_CONV >>
+  qexists_tac`next_addr bs.inst_length (TAKE (LENGTH bc0) bs.code)` >>
+  simp[RIGHT_EXISTS_AND_THM] >>
+  conj_tac >- (
+    match_mp_tac bc_find_loc_aux_ALL_DISTINCT >>
+    qexists_tac`LENGTH bc0` >> rfs[] >>
+    simp[EL_APPEND1,EL_APPEND2,VfromListCode_def]) >>
+  simp[TAKE_APPEND1] >>
+  qho_match_abbrev_tac`∃bls. bc_next^* bs1 (bs2 bls) ∧ P bls` >>
+  `bc_fetch bs1 = SOME (Stack (PushInt 0))` by (
+    match_mp_tac bc_fetch_next_addr >>
+    simp[Abbr`bs1`] >>
+    qexists_tac`bc0 ++ [HD VfromListCode]` >>
+    simp[VfromListCode_def,SUM_APPEND,FILTER_APPEND] ) >>
+  srw_tac[DNF_ss][Once RTC_CASES1] >> disj2_tac >>
+  simp[bc_eval1_thm,bc_eval1_def] >>
+  simp[bc_eval_stack_def,bump_pc_def] >>
+  simp[Abbr`bs1`] >>
+  qho_match_abbrev_tac`∃bls. bc_next^* bs1 (bs2 bls) ∧ P bls` >>
+  qspec_then`vl`mp_tac VfromListCode_aux_correct >> simp[] >>
+  `bs1.code = bs.code` by simp[Abbr`bs1`] >>
+  disch_then(qspec_then`bs1`mp_tac) >> simp[] >>
+  disch_then(qspec_then`bc0++(TAKE 2 VfromListCode)`mp_tac) >> simp[] >>
+  simp[Once VfromListCode_def] >>
+  simp[Once VfromListCode_def] >>
+  simp[Once VfromListCode_def] >> rfs[] >>
+  simp[Abbr`bs1`] >>
+  disch_then(qspec_then`pp`mp_tac) >> simp[] >>
+  discharge_hyps >- (
+    simp[VfromListCode_def] >>
+    REWRITE_TAC[SUM_APPEND,FILTER_APPEND,MAP_APPEND] >>
+    simp[] ) >>
+  strip_tac >>
+  qexists_tac`bls` >> simp[] >>
+  qho_match_abbrev_tac`bc_next^* bs1 (bs2 bls)` >>
+  qmatch_assum_abbrev_tac`bc_next^* bs1' bs3` >>
+  `bs1' = bs1` by (
+    simp[Abbr`bs1`,Abbr`bs1'`,bc_state_component_equality] >>
+    simp[VfromListCode_def] >>
+    REWRITE_TAC[SUM_APPEND,FILTER_APPEND,MAP_APPEND] >>
+    EVAL_TAC >> simp[] ) >>
+  simp[Once RTC_CASES_RTC_TWICE] >>
+  qunabbrev_tac`bs1'`>>fs[] >> pop_assum kall_tac >>
+  HINT_EXISTS_TAC >> simp[Abbr`bs1`] >>
+  `bc_fetch bs3 = SOME (Stack (Cons2 vector_tag))` by (
+    match_mp_tac bc_fetch_next_addr >>
+    simp[Abbr`bs3`] >>
+    qexists_tac`bc0 ++ (TAKE 20 VfromListCode)` >>
+    simp[VfromListCode_def] >>
+    REWRITE_TAC[FILTER_APPEND,SUM_APPEND,MAP_APPEND] >>
+    EVAL_TAC >> simp[] ) >>
+  srw_tac[DNF_ss][Once RTC_CASES1] >> disj2_tac >>
+  simp[bc_eval1_thm,bc_eval1_def,Abbr`bs3`,bc_eval_stack_def,bump_pc_def] >>
+  fs[Abbr`P`] >> imp_res_tac LIST_REL_LENGTH >> simp[] >>
+  simp[TAKE_APPEND1,TAKE_LENGTH_ID_rwt,DROP_APPEND1,DROP_LENGTH_NIL_rwt] >>
+  qho_match_abbrev_tac`bc_next^* bs1 (bs2 bls)` >>
+  `bc_fetch bs1 = SOME Return` by (
+    match_mp_tac bc_fetch_next_addr >>
+    simp[Abbr`bs1`] >>
+    qexists_tac`bc0 ++ (FRONT VfromListCode)` >>
+    simp[VfromListCode_def] >>
+    REWRITE_TAC[FILTER_APPEND,SUM_APPEND,MAP_APPEND] >>
+    EVAL_TAC >> simp[] ) >>
+  match_mp_tac RTC_SUBSET >>
+  simp[bc_eval1_thm,bc_eval1_def,Abbr`bs1`,Abbr`bs2`,bump_pc_def])
+
 val prim1_to_bc_thm = store_thm("prim1_to_bc_thm",
   ``∀rd op ck s v1 s' v bs bc0 bc1 bce st bv1.
     (bs.code = bc0 ++ prim1_to_bc op ++ bc1) ∧
+    contains_primitives bs.code ∧
     (bs.pc = next_addr bs.inst_length bc0) ∧
     (CevalPrim1 op s v1 = (s', Rval v)) ∧
     Cv_bv (mk_pp rd (bs with code := bce)) v1 bv1 ∧
@@ -1432,11 +1712,34 @@ val prim1_to_bc_thm = store_thm("prim1_to_bc_thm",
     match_mp_tac bc_fetch_next_addr >>
     map_every qexists_tac[`bc0`,`(TL (prim1_to_bc op)) ++ bc1`] >>
     Cases_on`op`>>rw[] ) >>
+  Cases_on`op = CVfromList` >- (
+    fs[] >> rw[] >>
+    Cases_on`CvFromList v1`>>fs[]>>rw[]>>
+    qspec_then`bs`mp_tac VfromListCode_correct >>
+    simp[] >>
+    disch_then(qspec_then`v1`mp_tac)>>simp[]>>
+    qmatch_assum_abbrev_tac`Cv_bv pp v1 bv1` >>
+    disch_then(qspec_then`pp`mp_tac)>>simp[]>>
+    strip_tac >>
+    simp[Cv_bv_cases_vectorv,PULL_EXISTS] >>
+    map_every qexists_tac[`bs.refs`,`bs.globals`,`rd.sm`,`bls`] >>
+    simp[] >>
+    conj_tac >- (
+      qmatch_assum_abbrev_tac`bc_next^* bs bs1` >>
+      qmatch_abbrev_tac`bc_next^* bs bs1'` >>
+      `bs1 = bs1'` by (
+        simp[Abbr`bs1`,Abbr`bs1'`] >>
+        simp[bump_pc_def,bc_state_component_equality] >>
+        simp[SUM_APPEND,FILTER_APPEND] ) >>
+      rw[] ) >>
+    match_mp_tac s_refs_with_irr >>
+    HINT_EXISTS_TAC >> simp[]) >>
   simp[Once RTC_CASES1] >>
   srw_tac[DNF_ss][] >> disj2_tac >>
   simp[bc_eval1_thm] >>
   PairCases_on`s` >>
-  Cases_on`op`>>simp[bc_eval1_def,bump_pc_def,bc_fetch_with_stack,bc_fetch_with_refs] >>
+  Cases_on`op`>>
+  simp[bc_eval1_def,bump_pc_def,bc_fetch_with_stack,bc_fetch_with_refs] >>
   fs[LET_THM] >- (
     qmatch_assum_abbrev_tac`CLoc n = v` >>
     simp[Once RTC_CASES1] >> srw_tac[DNF_ss][] >> disj2_tac >>
@@ -1590,7 +1893,7 @@ val prim1_to_bc_thm = store_thm("prim1_to_bc_thm",
     match_mp_tac s_refs_with_irr >>
     HINT_EXISTS_TAC >> simp[] )
   >- ((*LengthBlock*)
-    Cases_on`v1`>>fs[Cv_bv_cases_conv]>>
+    Cases_on`v1`>>fs[Cv_bv_cases_conv,Cv_bv_cases_vectorv]>>
     simp[bc_eval_stack_def] >>
     srw_tac[DNF_ss][Once RTC_CASES1] >> disj1_tac >>
     simp[bc_state_component_equality,FILTER_APPEND,SUM_APPEND] >>
